A general update. Now lisp_finalTheory produces assembly files containing the verified LISP interpeteres (in machine code):
  arm_eval.s
  x86_eval.s
  ppc_eval.s

Each of these have been successfully run on real hardware, for 
each respective platform.

The proof scripts are likely to only work in the experimental 
kernel, due to some unfortuante differences between the two 
kernels. Some of these differences are exposed more frequently 
now due to recent(ish) changes to the datatype package. Maybe 
some of the changes made to the datatype package ought to be 
reconsidered?

examples/machine-code/compiler/codegenLib.sml
@@ -285,9 +285,15 @@ fun add_assignment (tm1,tm2,th,len) = let
   val ws = pairSyntax.list_mk_pair (map snd ys)
   val tm3 = pairSyntax.mk_anylet([(vs,ws)],tm2)
   val lemma = prove(mk_eq(q,tm3),
-    SPEC_TAC (ws,genvar(type_of ws))
+    SIMP_TAC std_ss [LET_DEF]
+    THEN SPEC_TAC (ws,genvar(type_of ws))
     THEN SIMP_TAC std_ss [pairTheory.FORALL_PROD,LET_DEF]
-    THEN (fn x => hd [])) handle e => TRUTH
+    THEN (fn t => hd [])) handle e => TRUTH 
+(* (SPEC_TAC (ws,genvar(type_of ws))
+    THEN SIMP_TAC std_ss [pairTheory.FORALL_PROD,LET_DEF]
+    THEN NO_TAC) 
+   ORELSE SIMP_TAC std_ss [LET_DEF] 
+   ORELSE (fn t => hd [])) handle e => TRUTH *)
   val th = CONV_RULE (RAND_CONV (ONCE_REWRITE_CONV [lemma])) th
   val _ = add_decompiled (name,th,len,SOME len)
   in () end;
