examples/machine-code/lisp/export_codeLib.sig
@@ -1,0 +1,8 @@
+signature export_codeLib =
+sig
+
+    include Abbrev
+
+    val write_code_to_file   : string -> thm -> unit
+
+end
